{"nbformat":4,"nbformat_minor":0,"metadata":{"colab":{"name":"58089_PrelimPS_Pionelo.ipynb","provenance":[{"file_id":"https://github.com/dyjdlopez/fund-of-aiml/blob/main/activities/02%20-%20Linear%20Algebra%20Review/fund_aiml_02v1_2021.ipynb","timestamp":1631976839614}]},"kernelspec":{"name":"python3","display_name":"Python 3"},"language_info":{"name":"python"}},"cells":[{"cell_type":"markdown","metadata":{"id":"fte_zsqVdp8R"},"source":["# Topic02a : Prelim Problem Set I"]},{"cell_type":"markdown","metadata":{"id":"JpcY5oJ5eFxA"},"source":["##**Problem 1.a. System of Linear Equations**\n","$$ \\begin{bmatrix} z \\\\ y\\end{bmatrix} = \\begin{bmatrix} 0 \\\\ -\\frac{1}{32} \\end{bmatrix} + t\\begin{bmatrix} 1 \\\\ 1 \\end{bmatrix} $$\n","\n","$$ \\begin{bmatrix} x \\\\ y\\end{bmatrix} = \\begin{bmatrix} 0 \\\\0 \\end{bmatrix} + t\\begin{bmatrix} 4 \\\\ 1 \\end{bmatrix} $$\n","\n","$$ \\begin{bmatrix} x \\\\ z\\end{bmatrix} = \\begin{bmatrix} 3 \\\\ 7 \\end{bmatrix} + t\\begin{bmatrix} 0 \\\\ \\frac{28}{35} \\end{bmatrix}$$\n","##**Problem 1.b. Linear Combination**\n","$$ \\begin{bmatrix} \\cos({\\theta}) & sin({\\theta}) & -csc({2\\theta}) \\end{bmatrix}\\cdot \\begin{bmatrix} \\hat{i} \\\\ \\hat{j} \\\\ \\hat{k} \\end{bmatrix} = \\begin{bmatrix} \\cos{(\\theta)}\\hat{i} & sin{(\\theta)}\\hat{j} & -csc{(2\\theta)}\\hat{k}  \\end{bmatrix}$$\n","##**Problem 1.c. Scenario**\n","$$  Students (x):  \\frac{200}{260} \\times 100  =  76.92\\% $$\n","\n","$$ Professionals (y):  \\frac{45}{260} \\times 100  =  17.31\\% $$\n","\n","$$ Panel (z):  \\frac{15}{260} \\times 100  =  5.77\\% $$\n","\n","\n","$$ 100 \\times \\begin{bmatrix} \\frac{10}{13} & \\frac{9}{52} & \\frac{1}{52} \\end{bmatrix} \\cdot \\begin{bmatrix} x \\\\ y\\\\ z \\end{bmatrix}  =  \\begin{bmatrix} 76.92\\% x & 17.31\\%y & 5.77\\%z \\end{bmatrix}$$"]},{"cell_type":"markdown","metadata":{"id":"Uvb1MGs9QNVt"},"source":["##**Problem 2.a: Vector Magnitude**<br>\n","The magnitude of a vector has a given formula which is\n","$$||v|| = \\sqrt{a_0^2 + a_1^2 + ... +a_n^2}$$\n","\n","But since the dot product of the vector $v$ is equal to the dot product of the same vector $v$\n","$$v\\cdot v = \\begin{bmatrix} a_0 \\\\ a_1 \\\\ \\vdots \\\\ a_n \\end{bmatrix}\\cdot \\begin{bmatrix} a_0 \\\\ a_1 \\\\ \\vdots \\\\ a_n \\end{bmatrix}$$\n","\n","We can say that the dot product of vector $v$ is equal to \n","$${a_0^2 + a_1^2 + ... +a_n^2}$$\n","<br>\n","Which means that the usual formula $||v|| = \\sqrt{a_0^2 + a_1^2 + ... +a_n^2}$ is equal to\n","\n","$$||v|| = \\sqrt{v \\cdot v}\\\\ or \\\\||v||^2 = v \\cdot v$$\n","\n","##**Problem 2.b: Angle Between Vectors**\n","Two vectors are $\\textrm{orthogonal}$ if the two vectors are *perpendicular* to each other or if they dot product of the two vectors is *zero*.\n","\n","For example,\n","$$v = \\begin{bmatrix}1 \\\\ \\sqrt2 \\\\ 1\\end{bmatrix}, u = \\begin{bmatrix}1 \\\\ -\\sqrt2 \\\\ 1\\end{bmatrix}$$\n","\n","$$v \\cdot u =\\begin{bmatrix}1 & \\sqrt2 & 1\\end{bmatrix} \\cdot \\begin{bmatrix}1 & -\\sqrt2 & 1\\end{bmatrix}$$\n","$$v \\cdot u = 1(1) + \\sqrt{2}(-\\sqrt{2})+1(1)$$\n","$$v \\cdot u = 1 -2 + 1 = 0$$\n","\n","Since the dot product $v\\cdot u$ is equal to 0, the vectors $v$ and $u$ is $\\textrm{orthogonal}$. (Perpendicular) <br><br>\n","\n","Two vectors are $parallel$ if their angle $\\theta$ is equal to $0^{\\circ}$ or $180^{\\circ}$ following the formula $$\\theta = cos^{-1}\\begin{bmatrix}\\frac{ A\\cdot B}{||A||\\cdot ||B||}\\end{bmatrix}$$\n","\n","For example,\n","$$v = \\begin{bmatrix}4 \\\\ 3\\end{bmatrix}, u = \\begin{bmatrix}12 \\\\ 9\\end{bmatrix}$$\n","\n","$$v \\cdot u = 4(12) + 3(9) = 48 + 27 = 75$$\n","\n","$$||v|| = \\sqrt{4^2 + 3^2}= \\sqrt{16 + 9} = 5$$\n","\n","$$||u|| = \\sqrt{12^2 + 9^2}= \\sqrt{144 + 81} = 15$$\n","\n","$$\\theta = cos^{-1}\\begin{bmatrix}\\frac{75}{5\\cdot 15}\\end{bmatrix}$$\n","\n","$$\\theta = cos^{-1}\\begin{bmatrix}\\frac{75}{75}\\end{bmatrix}$$\n","\n","$$\\theta = cos^{-1}(1)$$\n","$$\\theta = 0^{\\circ}$$\n","\n","Since the angle $\\theta$ of the two vectors is equal to $0^{\\circ}$, the two vectors are $parallel$ to each other."]},{"cell_type":"markdown","metadata":{"id":"MQ8jJV9-qyFy"},"source":["## **Problem 3.a: Matrix Equivalences**\n","\n","The matrix multiplication $\\theta^T\\cdot X$ can also be defined as a table of dot products between all pairs of the two vectors $X$ and $\\theta$.\n","\n","Considering that $X$ and $\\theta$ has matrix of:\n","\n","$$X = \\begin{bmatrix} \n","— (x^{(1)})^T— \\\\ \n","— (x^{(2)})^T— \\\\\n","\\vdots \\\\\n","— (x^{(m)})^T— \\\\\n","\\end{bmatrix} \\text{, and }\n","\\theta = \\begin{bmatrix} \n","\\theta^{(1)} \\\\ \n","\\theta^{(2)} \\\\\n","\\vdots \\\\\n","\\theta^{(m)} \\\\\n","\\end{bmatrix}$$\n","Since,\n","\n","$$v^Tw=\\begin{bmatrix}v_1 \\cdots v_n\\end{bmatrix}\\begin{bmatrix}w_1 \\\\ \\vdots \\\\ w_n\\end{bmatrix} = v_1w_1+\\dots+v_nw_n = v\\cdot w$$\n","\n","Then,\n","$$\\theta^TX = \\begin{bmatrix}\\theta^{(1)} & \\theta^{(2)} & \\dots & \\theta^{(m)} \\\\\\end{bmatrix} \\begin{bmatrix} (x^{(1)})^T \\\\ (x^{(2)})^T \\\\ \\vdots \\\\ (x^{(m)})^T \\\\ \\end{bmatrix} = \\theta^{(1)}(x^{(1)})^T+\\theta^{(2)}(x^{(2)})^T+\\dots+\\theta^{(m)}(x^{(m)})^T = X \\cdot \\theta$$\n","\n","$$\\theta^TX=X\\cdot\\theta$$\n","\n","##**Problem 3.b: Matrix Shapes**\n","\n","$$X = \\begin{bmatrix} \n"," a^{(1)} & a^{(2)} & a^{(3)} & a^{(4)} & a^{(5)}\\\\ \n","a^{(6)} & a^{(7)} & a^{(8)} & a^{(9)} & a^{(10)} \\\\\n","\\vdots & \\vdots & \\vdots & \\vdots & \\vdots\\\\\n","a^{(296)} & a^{(297)} & a^{(298)} & a^{(299)} & a^{(300)}\n","\\\\\n","\\end{bmatrix}  ,\\theta = \\begin{bmatrix} \n","\\theta^{(1)} \\\\ \n","\\theta^{(2)} \\\\\n","\\vdots \\\\\n","\\theta^{(k)} \\\\\n","\\end{bmatrix} $$\n","\\\n","$$g(z) = \\frac{1}{1+e^{-z}}$$\n","\\\n","Since,\n","\\\n"," $$z = X \\cdot \\theta$$\n","Then,  $$ h_\\theta(x) = g(X \\cdot \\theta)$$\n","\\\n","$$h_\\theta(x) = g(z)$$\n","\\\n","Applying $(k \\cdot 1)$ and $(m \\cdot k)$, we get $z$. The $z$ will then be passed to the sigmoid function, and the final result will be $ h_\\theta(x)$. The equation can be merge into one therefore the $ h_\\theta(x)$ would have the same matrix shape as $X$ \n","\\\n","\\\n","$$ h_\\theta(x) = \\begin{bmatrix} \n"," \\theta^1{(a)} & \\theta^2{(a)} & \\theta^3{(a)} & \\theta^4{(a)} & \\theta^5{(a)}\\\\ \n","\\theta^6{(a)} & \\theta^7{(a)} & \\theta^8{(a)} & \\theta^9{(a)} & \\theta^{10} {(a)}\\\\\n","\\vdots & \\vdots & \\vdots & \\vdots & \\vdots\\\\\n","\\theta^{296}{(a)} & \\theta^{297}{(a)} & \\theta^{298}{(a)} & \\theta^{299}{(a)} & \\theta^{300}{(a)}\\\\  \\end{bmatrix}$$\n","\\\n","${\\therefore}$ The shape of  $h_\\theta$ is $(300, 5)$\n","\n","##**Problem 3.c: Vectorization**\n","\n","Given:\n","$$J(\\theta) = \\frac{1}{m} \\sum^m_{i=0}=[-y^{(i)}\\log({h_{\\theta}(x^{(i)})})-(1-y^{(i)})\\log(1-h_{\\theta}(x^{(i)}))]$$\n","\n","Considering that\n","\n","$$(\\log({h_{\\theta}(x)})-(1-y)\\log(1-h_{\\theta}(x))) = \\begin{bmatrix}(\\log({h_{\\theta}(x^{(1)})})-(1-y^{(1)})\\log(1-h_{\\theta}(x^{(1)}))) \\\\ (\\log({h_{\\theta}(x^{(2)})})-(1-y^{(2)})\\log(1-h_{\\theta}(x^{(2)}))) \\\\ \\vdots \\\\ (\\log({h_{\\theta}(x^{(3)})})-(1-y^{(3)})\\log(1-h_{\\theta}(x^{(3)})))\\end{bmatrix}$$\n","\n","Then\n","\n","$$\\begin{bmatrix}J(\\theta)_0 \\\\ J(\\theta)_1 \\\\ \\vdots \\\\ J(\\theta)_n \\end{bmatrix} = \\frac{1}{m}\\begin{bmatrix}\\sum^m_{i=0}(-y^{(i)}_0\\log({h_{\\theta}(x^{(i)})})-(1-y^{(i)})\\log(1-h_{\\theta}(x^{(i)}))) \\\\ \\sum^m_{i=0}(-y^{(i)}_1\\log({h_{\\theta}(x^{(i)})})-(1-y^{(i)})\\log(1-h_{\\theta}(x^{(i)}))) \\\\ \\vdots \\\\ \\sum^m_{i=0}(-y^{(i)}_n\\log({h_{\\theta}(x^{(i)})})-(1-y^{(i)})\\log(1-h_{\\theta}(x^{(i)})))\\end{bmatrix}$$\n","\n","$$\\begin{bmatrix}J(\\theta)_0 \\\\ J(\\theta)_1 \\\\ \\vdots \\\\ J(\\theta)_n \\end{bmatrix} = \\frac{1}{m}\\sum^m_{i=0} (-y^{(i)}\\log({h_{\\theta}(x^{(i)})})-(1-y^{(i)})\\log(1-h_{\\theta}(x^{(i)})))$$\n","\n","$$\\begin{bmatrix}J(\\theta)_0 \\\\ J(\\theta)_1 \\\\ \\vdots \\\\ J(\\theta)_n \\end{bmatrix} = \\frac{1}{m}(-Y^T)(\\log({h_{\\theta}(x)})-(1-y)\\log(1-h_{\\theta}(x)))$$\n","\n","$$\\text{Let }\\beta_i = (log(h_\\theta(x^{(i)}))-(1-y^{(i)})log(1-h_\\theta(x^{(i)})))$$\n","\n","$$\\sum_i\\beta_i(-y^{(i)})=\\begin{bmatrix}y^{(1)} & y^{(2)} & \\cdots & y^{(m)}\\end{bmatrix}\\begin{bmatrix}\\beta_1 \\\\ \\beta_2 \\\\ \\vdots \\\\ \\beta_m\\end{bmatrix} = -Y^T\\beta$$\n","##**Problem 4.c: Computational Programming (Also Laboratory 2)**"]}]}