{"nbformat":4,"nbformat_minor":0,"metadata":{"colab":{"name":"*section*_PrelimPS_*name*.ipynb","provenance":[{"file_id":"https://github.com/dyjdlopez/fund-of-aiml/blob/main/activities/02%20-%20Linear%20Algebra%20Review/fund_aiml_02v1_2021.ipynb","timestamp":1631527913285}],"collapsed_sections":[]},"kernelspec":{"name":"python3","display_name":"Python 3"},"language_info":{"name":"python"}},"cells":[{"cell_type":"markdown","metadata":{"id":"fte_zsqVdp8R"},"source":["# Topic02a : Prelim Problem Set I\n"]},{"cell_type":"markdown","metadata":{"id":"vo_c4LChv_8w"},"source":["## **Case 1**\n","\n","### **Problem 1.a System of Linear Equations**\n","\n","$$ \\begin{bmatrix} z \\\\ y\\end{bmatrix} = \\begin{bmatrix} 0 \\\\ -\\frac{1}{32} \\end{bmatrix} + t\\begin{bmatrix} 1 \\\\ 1 \\end{bmatrix} $$ \n","\n","$$ \\begin{bmatrix} x \\\\ y\\end{bmatrix} = \\begin{bmatrix} 0 \\\\0 \\end{bmatrix} + t\\begin{bmatrix} 4 \\\\ 1 \\end{bmatrix} $$\n","\n","$$ \\begin{bmatrix} x \\\\ z\\end{bmatrix} = \\begin{bmatrix} 3 \\\\ 7 \\end{bmatrix} + t\\begin{bmatrix} 0 \\\\ \\frac{28}{35} \\end{bmatrix}$$\n","\n","\n","### **Problem 1.b Linear Combination**\n","\n","\n","$$ \\begin{bmatrix} \\cos{(\\theta)} & sin{(\\theta)} & -csc{(2\\theta)}  \\end{bmatrix} \\cdot \\begin{bmatrix} \\hat{i} \\\\ \\hat{j} \\\\ \\hat{k} \\end{bmatrix} = \\begin{bmatrix} \\cos{(\\theta)}\\hat{i} & sin{(\\theta)}\\hat{j} & -csc{(2\\theta)}\\hat{k}  \\end{bmatrix}$$\n","\n","\n","### **Problem 1.c Scenario**\n","\n","Problem 1.c Scenario\n","\n","$$  Students = (x) =  \\frac{200}{260} \\times 100  =  76.92\\% $$\n","\n","$$ Professionals = (y) =  \\frac{45}{260} \\times 100  =  17.31\\% $$\n","\n","$$ Panel = (z) =  \\frac{15}{260} \\times 100  =  5.77\\% $$\n","\n","\n","$$ 100 \\times \\begin{bmatrix} \\frac{10}{13} & \\frac{9}{52} & \\frac{1}{52} \\end{bmatrix} \\cdot \\begin{bmatrix} x \\\\ y\\\\ z \\end{bmatrix}  =  \\begin{bmatrix} 76.92\\% x & 17.31\\%y & 5.77\\%z \\end{bmatrix}$$\n","\n"]},{"cell_type":"markdown","metadata":{"id":"RjjOcqDRcM2t"},"source":["## **Case 2**\n","\n","###**Problem 2.a: Vector Magnitude**\n","\n","Usual Formula:\n","$$||v|| = \\sqrt{a_0^2 + a_1^2 + ... +a_n^2}$$\n","\n","Function of a Inner product on a space of all continuous functions on the closed interval from a to b\n","\n","$$||v|| = \\sqrt{\\langle v|v \\rangle} = \\sqrt{\\int_{a}^{b} v^2(x) \\,dx} $$\n","\n","\n","\\\\\n","\n","For getting the magnitude/length/norm of a vector, the usual formula used is the $$||v|| = \\sqrt{a_0^2 + a_1^2 + ... +a_n^2}$$ \n","which $||v||$ value is also called the Euclendian norm or $l_2-norm$ based on the formula (using $v$ to represent any vector):  $$||v|| = ||v||_p = (\\sum_{i=1}^n {|v_i|}^p)^{\\frac{1}{p}} $$ where $p = 2$\n"," \\\\\n","\n","A norm in the Inner Product Space and continuous function (from a to b) space be represented as: \n","\n","$$ ||v|| = {\\langle v|v \\rangle}  = \\int_{a}^{b} v^2(x) \\,dx$$ \n","\n","and since the given is a Eucledian Norm, the usual formula reformuled as a function of a inner product would look like this \n","\n","$$||v|| = \\sqrt{\\langle v|v \\rangle} = \\sqrt{\\int_{a}^{b} v^2(x) \\,dx} $$ or \n","\n","\n","\n","\n","$$||v|| = \\sqrt{\\langle v|v \\rangle} = [\\int_{a}^{b} v^2(x) \\,dx]^\\frac{1}{2} $$\n","\n","\n","\n","\n","\n","\n","\n","\n","### **Problem 2.b**\n","\n","The dot product of $||u||$ , $||v||$ , and  $\\cos(\\theta)$ with $\\theta = 90^\\circ$ or $270^\\circ$  would produce a result of $0$ since both non zero vectors $u$ and $v$ are perpendicular to each other and $\\cos{90} = {0}$. The dot product of a not zero vector to zero vector is equal to zero.\n","\n","$$u\\cdot v =||u||\\cdot||v||cos({90}) / u\\cdot v =||u||\\cdot||v||cos({270})$$ \n","$$u\\cdot v =(||u||\\cdot||v||)(0)$$\n","$$u\\cdot v = 0$$\n","\n","Therefore, Vector $u$ is **Orthological** or **Perpendicular** to Vector $v$.\n","\n","\n","\n","\\\\\n","The dot product of  $||u||$ , $||v||$ , and  $\\cos(\\theta)$ with $\\theta = 0^\\circ$ would produce a positive output that is the dot product of vectors $u$ and $v$ since $\\cos{0} = {1}$. If $\\theta = 180^\\circ$, then it would produce a negative dot product output of vectors $u$ and $v$ as $cos(180) = -1$. \n","\\\\ $$\\theta = 0^\\circ$$\n","$$u\\cdot v =||u||\\cdot||v||cos({0})$$ \n","$$u\\cdot v =(||u||\\cdot||v||)(1)$$\n","$$u\\cdot v = ||u||\\cdot||v||$$ \\\\\n","\n","$$\\theta = 180^\\circ$$\n","$$u\\cdot v =||u||\\cdot||v||cos{180}$$ \n","$$u\\cdot v =(||u||\\cdot||v||)(-1)$$\n","$$u\\cdot v = -(||u||\\cdot||v||)$$\n","\n"]},{"cell_type":"markdown","metadata":{"id":"lWT4Y-4hzVUO"},"source":["## **Case 3**\n","\n","###**Problem 3.a: Matrix Equivalences**\n","\n","The matrix multiplication $\\theta^T\\cdot X$ can also be defined as a table of dot products between all pairs of the two vectors $X$ and $\\theta$.\n","\n","Considering that $X$ and $\\theta$ has matrix of:\n","\n","$$X = \\begin{bmatrix} \n","— (x^{(1)})^T— \\\\ \n","— (x^{(2)})^T— \\\\\n","\\vdots \\\\\n","— (x^{(m)})^T— \\\\\n","\\end{bmatrix} \\text{, and }\n","\\theta = \\begin{bmatrix} \n","\\theta^{(1)} \\\\ \n","\\theta^{(2)} \\\\\n","\\vdots \\\\\n","\\theta^{(m)} \\\\\n","\\end{bmatrix}$$\n","Since,\n","\n","$$v^Tw=\\begin{bmatrix}v_1 \\cdots v_n\\end{bmatrix}\\begin{bmatrix}w_1 \\\\ \\vdots \\\\ w_n\\end{bmatrix} = v_1w_1+\\dots+v_nw_n = v\\cdot w$$\n","\n","Then,\n","$$\\theta^TX = \\begin{bmatrix}\\theta^{(1)} & \\theta^{(2)} & \\dots & \\theta^{(m)} \\\\\\end{bmatrix} \\begin{bmatrix} (x^{(1)})^T \\\\ (x^{(2)})^T \\\\ \\vdots \\\\ (x^{(m)})^T \\\\ \\end{bmatrix} = \\theta^{(1)}(x^{(1)})^T+\\theta^{(2)}(x^{(2)})^T+\\dots+\\theta^{(m)}(x^{(m)})^T = X \\cdot \\theta$$\n","\n","$$\\theta^TX=X\\cdot\\theta$$\n","###**Problem 3.b: Matrix Shapes**\n","$$X = \\begin{bmatrix} \n"," a^{(1)} & a^{(2)} & a^{(3)} & a^{(4)} & a^{(5)}\\\\ \n","a^{(6)} & a^{(7)} & a^{(8)} & a^{(9)} & a^{(10)} \\\\\n","\\vdots & \\vdots & \\vdots & \\vdots & \\vdots\\\\\n","a^{(296)} & a^{(297)} & a^{(298)} & a^{(299)} & a^{(300)}\n","\\\\\n","\\end{bmatrix}  ,\\theta = \\begin{bmatrix} \n","\\theta^{(1)} \\\\ \n","\\theta^{(2)} \\\\\n","\\vdots \\\\\n","\\theta^{(k)} \\\\\n","\\end{bmatrix} $$\n","\\\n","$$g(z) = \\frac{1}{1+e^{-z}}$$\n","\\\n","Since,\n","\\\n"," $$z = X \\cdot \\theta$$\n","Then,  $$ h_\\theta(x) = g(X \\cdot \\theta)$$\n","\\\n","$$h_\\theta(x) = g(z)$$\n","\\\n","Applying $(k \\cdot 1)$ and $(m \\cdot k)$, we get $z$. The $z$ will then be passed to the sigmoid function, and the final result will be $ h_\\theta(x)$. The equation can be merge into one therefore the $ h_\\theta(x)$ would have the same matrix shape as $X$ \n","\\\n","\\\n","$$ h_\\theta(x) = \\begin{bmatrix} \n"," \\theta^1{(a)} & \\theta^2{(a)} & \\theta^3{(a)} & \\theta^4{(a)} & \\theta^5{(a)}\\\\ \n","\\theta^6{(a)} & \\theta^7{(a)} & \\theta^8{(a)} & \\theta^9{(a)} & \\theta^{10} {(a)}\\\\\n","\\vdots & \\vdots & \\vdots & \\vdots & \\vdots\\\\\n","\\theta^{296}{(a)} & \\theta^{297}{(a)} & \\theta^{298}{(a)} & \\theta^{299}{(a)} & \\theta^{300}{(a)}\\\\  \\end{bmatrix}$$\n","\\\n","${\\therefore}$ The shape of  $h_\\theta$ is $(300, 5)$"]},{"cell_type":"markdown","metadata":{"id":"FCikQY-EYhes"},"source":["###**Problem 3.c: Vectorization**\n","Given:\n","$$J(\\theta) = \\frac{1}{m} \\sum^m_{i=0}=[-y^{(i)}\\log({h_{\\theta}(x^{(i)})})-(1-y^{(i)})\\log(1-h_{\\theta}(x^{(i)}))]$$\n","\n","Considering that\n","\n","$$(\\log({h_{\\theta}(x)})-(1-y)\\log(1-h_{\\theta}(x))) = \\begin{bmatrix}(\\log({h_{\\theta}(x^{(1)})})-(1-y^{(1)})\\log(1-h_{\\theta}(x^{(1)}))) \\\\ (\\log({h_{\\theta}(x^{(2)})})-(1-y^{(2)})\\log(1-h_{\\theta}(x^{(2)}))) \\\\ \\vdots \\\\ (\\log({h_{\\theta}(x^{(3)})})-(1-y^{(3)})\\log(1-h_{\\theta}(x^{(3)})))\\end{bmatrix}$$\n","\n","Then\n","\n","$$\\begin{bmatrix}J(\\theta)_0 \\\\ J(\\theta)_1 \\\\ \\vdots \\\\ J(\\theta)_n \\end{bmatrix} = \\frac{1}{m}\\begin{bmatrix}\\sum^m_{i=0}(-y^{(i)}_0\\log({h_{\\theta}(x^{(i)})})-(1-y^{(i)})\\log(1-h_{\\theta}(x^{(i)}))) \\\\ \\sum^m_{i=0}(-y^{(i)}_1\\log({h_{\\theta}(x^{(i)})})-(1-y^{(i)})\\log(1-h_{\\theta}(x^{(i)}))) \\\\ \\vdots \\\\ \\sum^m_{i=0}(-y^{(i)}_n\\log({h_{\\theta}(x^{(i)})})-(1-y^{(i)})\\log(1-h_{\\theta}(x^{(i)})))\\end{bmatrix}$$\n","\n","$$\\begin{bmatrix}J(\\theta)_0 \\\\ J(\\theta)_1 \\\\ \\vdots \\\\ J(\\theta)_n \\end{bmatrix} = \\frac{1}{m}\\sum^m_{i=0} (-y^{(i)}\\log({h_{\\theta}(x^{(i)})})-(1-y^{(i)})\\log(1-h_{\\theta}(x^{(i)})))$$\n","\n","$$\\begin{bmatrix}J(\\theta)_0 \\\\ J(\\theta)_1 \\\\ \\vdots \\\\ J(\\theta)_n \\end{bmatrix} = \\frac{1}{m}(-Y^T)(\\log({h_{\\theta}(x)})-(1-y)\\log(1-h_{\\theta}(x)))$$\n","\n","$$\\text{Let }\\beta_i = (log(h_\\theta(x^{(i)}))-(1-y^{(i)})log(1-h_\\theta(x^{(i)})))$$\n","\n","$$\\sum_i\\beta_i(-y^{(i)})=\\begin{bmatrix}y^{(1)} & y^{(2)} & \\cdots & y^{(m)}\\end{bmatrix}\\begin{bmatrix}\\beta_1 \\\\ \\beta_2 \\\\ \\vdots \\\\ \\beta_m\\end{bmatrix} = -Y^T\\beta$$"]},{"cell_type":"markdown","metadata":{"id":"_X1fHHaJYpLd"},"source":["###**Problem 4.c: Computational Programming (Also Laboratory 2)**"]}]}